Finished Encrypt verification
fix: Finished all required encrypt verification
chore: Removed all requirements which where not part of the client from the client
chore: Added part of the verification to the corresponding files

src/SDK/CMM/Defs.dfy
@@ -24,7 +24,7 @@ module {:extern "CMMDefs"} CMMDefs {
       ensures Valid()
       ensures res.Success? ==> EncryptionMaterialsSignature(res.value)
       ensures res.Success? ==> res.value.plaintextDataKey.Some? && res.value.Serializable()
-      
+
     // The following predicate is a synonym for Encryption.Serializable and provides a workaround for a translation bug
     // of "fuel" in trait-override checks in Dafny. https://github.com/dafny-lang/dafny/issues/422
     static predicate ValidAAD(encryptionContext: EncryptionContext.Map) {
@@ -38,7 +38,12 @@ module {:extern "CMMDefs"} CMMDefs {
       ensures res.Success? ==> res.value.plaintextDataKey.Some?
   }
 
-  predicate {:opaque } EncryptionMaterialsSignature(validEncryptionMaterials: Materials.ValidEncryptionMaterials)
+  // Predicate works arround a known error in Dafny: https://github.com/dafny-lang/dafny/issues/422 
+  predicate EncryptionMaterialsSignature(validEncryptionMaterials: Materials.ValidEncryptionMaterials) {
+    EncryptionMaterialsSignatureOpaque(validEncryptionMaterials)
+  }
+
+  predicate {:opaque } EncryptionMaterialsSignatureOpaque(validEncryptionMaterials: Materials.ValidEncryptionMaterials)
     {
       true
     }
